barrier/lifting.v
@@ -1,5 +1,5 @@
 Require Export barrier.parameter.
-Require Import prelude.gmap iris.lifting.
+Require Import prelude.gmap iris.lifting barrier.heap_lang.
 Import uPred.
 
 (* TODO RJ: Figure out a way to to always use our Σ. *)
@@ -11,7 +11,35 @@ Proof.
   by apply (wp_bind (Σ:=Σ) (K := fill K)), fill_is_ctx.
 Qed.
 
-(** Base axioms for core primitives of the language. *)
+(** Base axioms for core primitives of the language: Stateful reductions *)
+
+Lemma wp_lift_step E1 E2 (φ : expr → state → Prop) Q e1 σ1 :
+  E1 ⊆ E2 → to_val e1 = None →
+  reducible e1 σ1 →
+  (∀ e2 σ2 ef, prim_step e1 σ1 e2 σ2 ef → ef = None ∧ φ e2 σ2) →
+  pvs E2 E1 (ownP (Σ:=Σ) σ1 ★ ▷ ∀ e2 σ2, (■ φ e2 σ2 ∧ ownP (Σ:=Σ) σ2) -★
+    pvs E1 E2 (wp (Σ:=Σ) E2 e2 Q))
+  ⊑ wp (Σ:=Σ) E2 e1 Q.
+Proof.
+  (* RJ FIXME WTF the bound names of wp_lift_step *changed*?!?? *)
+  intros ? He Hsafe Hstep.
+  etransitivity; last eapply wp_lift_step with (σ2 := σ1)
+    (φ0 := λ e' σ' ef, ef = None ∧ φ e' σ'); last first.
+  - intros e2 σ2 ef Hstep'%prim_ectx_step; last done.
+    by apply Hstep.
+  - destruct Hsafe as (e' & σ' & ? & ?).
+    do 3 eexists. exists EmptyCtx. do 2 eexists.
+    split_ands; try (by rewrite fill_empty); eassumption.
+  - done.
+  - eassumption.
+  - apply pvs_mono. apply sep_mono; first done.
+    apply later_mono. apply forall_mono=>e2. apply forall_mono=>σ2.
+    apply forall_intro=>ef. apply wand_intro_l.
+    rewrite always_and_sep_l' -associative -always_and_sep_l'.
+    apply const_elim_l; move=>[-> Hφ]. eapply const_intro_l; first eexact Hφ.
+    rewrite always_and_sep_l' associative -always_and_sep_l' wand_elim_r.
+    apply pvs_mono. rewrite right_id. done.
+Qed.
 
 (* TODO RJ: Figure out some better way to make the
    postcondition a predicate over a *location* *)
@@ -23,11 +51,9 @@ Lemma wp_alloc E σ v:
 Proof.
   (* RJ FIXME: rewrite would be nicer... *)
   etransitivity; last eapply wp_lift_step with (σ1 := σ)
-    (φ := λ e' σ' ef, ∃ l, e' = Loc l ∧ σ' = <[l:=v]>σ ∧ σ !! l = None ∧ ef = None);
+    (φ := λ e' σ', ∃ l, e' = Loc l ∧ σ' = <[l:=v]>σ ∧ σ !! l = None);
     last first.
-  - intros e2 σ2 ef Hstep%prim_ectx_step; last first.
-    { exists ∅. do 3 eexists. eapply AllocS with (l:=0); by rewrite ?v2v. }
-    inversion_clear Hstep.
+  - intros e2 σ2 ef Hstep. inversion_clear Hstep. split; first done.
     rewrite v2v in Hv. inversion_clear Hv.
     eexists; split_ands; done.
   - (* RJ FIXME: Need to find a fresh location. *) admit.
@@ -36,9 +62,9 @@ Proof.
   - (* RJ FIXME I am sure there is a better way to invoke right_id, but I could not find it. *)
     rewrite -pvs_intro. rewrite -{1}[ownP σ](@right_id _ _ _ _ uPred.sep_True).
     apply sep_mono; first done. rewrite -later_intro.
-    apply forall_intro=>e2. apply forall_intro=>σ2. apply forall_intro=>ef.
+    apply forall_intro=>e2. apply forall_intro=>σ2.
     apply wand_intro_l. rewrite right_id. rewrite -pvs_intro.
-    apply const_elim_l. intros [l [-> [-> [Hl ->]]]]. rewrite right_id.
+    apply const_elim_l. intros [l [-> [-> Hl]]].
     rewrite -wp_value'; last reflexivity.
     erewrite <-exist_intro with (a := l). apply and_intro.
     + by apply const_intro.
@@ -50,21 +76,17 @@ Lemma wp_load E σ l v:
   ownP (Σ:=Σ) σ ⊑ wp (Σ:=Σ) E (Load (Loc l)) (λ v', ■(v' = v) ∧ ownP (Σ:=Σ) σ).
 Proof.
   intros Hl. etransitivity; last eapply wp_lift_step with (σ1 := σ)
-    (φ := λ e' σ' ef, e' = v2e v ∧ σ' = σ ∧ ef = None); last first.
-  - intros e2 σ2 ef Hstep%prim_ectx_step; last first.
-    { exists σ. do 3 eexists. eapply LoadS; eassumption. }
-    move: Hl. inversion_clear Hstep=>{σ}. rewrite Hlookup.
-    case=>->. done.
-  - do 3 eexists. exists EmptyCtx. do 2 eexists.
-    split_ands; try (by rewrite fill_empty); [].
-    eapply LoadS; eassumption.
+    (φ := λ e' σ', e' = v2e v ∧ σ' = σ); last first.
+  - intros e2 σ2 ef Hstep. move: Hl. inversion_clear Hstep=>{σ}.
+    rewrite Hlookup. case=>->. done.
+  - do 3 eexists. eapply LoadS; eassumption.
   - reflexivity.
   - reflexivity.
   - rewrite -pvs_intro. rewrite -{1}[ownP σ](@right_id _ _ _ _ uPred.sep_True).
     apply sep_mono; first done. rewrite -later_intro.
-    apply forall_intro=>e2. apply forall_intro=>σ2. apply forall_intro=>ef.
+    apply forall_intro=>e2. apply forall_intro=>σ2.
     apply wand_intro_l. rewrite right_id. rewrite -pvs_intro.
-    apply const_elim_l. intros [-> [-> ->]]. rewrite right_id.
+    apply const_elim_l. intros [-> ->].
     rewrite -wp_value. apply and_intro.
     + by apply const_intro.
     + done.
@@ -72,25 +94,47 @@ Qed.
 
 Lemma wp_store E σ l v v':
   σ !! l = Some v' →
-  ownP (Σ:=Σ) σ ⊑ wp (Σ:=Σ) E (Store (Loc l) (v2e v)) (λ v', ■(v' = LitVUnit) ∧ ownP (Σ:=Σ) (<[l:=v]>σ)).
+  ownP (Σ:=Σ) σ ⊑ wp (Σ:=Σ) E (Store (Loc l) (v2e v))
+       (λ v', ■(v' = LitVUnit) ∧ ownP (Σ:=Σ) (<[l:=v]>σ)).
 Proof.
   intros Hl. etransitivity; last eapply wp_lift_step with (σ1 := σ)
-    (φ := λ e' σ' ef, e' = LitUnit ∧ σ' = <[l:=v]>σ ∧ ef = None); last first.
-  - intros e2 σ2 ef Hstep%prim_ectx_step; last first.
-    { exists σ. do 3 eexists. eapply StoreS; last (eexists; eassumption). by rewrite v2v. }
-    move: Hl. inversion_clear Hstep=>{σ2}. rewrite v2v in Hv. inversion_clear Hv.
-    done.
-  - do 3 eexists. exists EmptyCtx. do 2 eexists.
-    split_ands; try (by rewrite fill_empty); [].
-    eapply StoreS; last (eexists; eassumption). by rewrite v2v.
+    (φ := λ e' σ', e' = LitUnit ∧ σ' = <[l:=v]>σ); last first.
+  - intros e2 σ2 ef Hstep. move: Hl. inversion_clear Hstep=>{σ2}.
+    rewrite v2v in Hv. inversion_clear Hv. done.
+  - do 3 eexists. eapply StoreS; last (eexists; eassumption). by rewrite v2v.
   - reflexivity.
   - reflexivity.
   - rewrite -pvs_intro. rewrite -{1}[ownP σ](@right_id _ _ _ _ uPred.sep_True).
     apply sep_mono; first done. rewrite -later_intro.
-    apply forall_intro=>e2. apply forall_intro=>σ2. apply forall_intro=>ef.
+    apply forall_intro=>e2. apply forall_intro=>σ2.
     apply wand_intro_l. rewrite right_id. rewrite -pvs_intro.
-    apply const_elim_l. intros [-> [-> ->]]. rewrite right_id.
+    apply const_elim_l. intros [-> ->].
     rewrite -wp_value'; last reflexivity. apply and_intro.
     + by apply const_intro.
     + done.
+Qed.
+
+(** Base axioms for core primitives of the language: Stateless reductions *)
+
+Lemma wp_fork E e :
+  ▷ wp (Σ:=Σ) coPset_all e (λ _, True) ⊑ wp (Σ:=Σ) E (Fork e) (λ _, True).
+Proof.
+  etransitivity; last eapply wp_lift_pure_step with
+    (φ := λ e' ef, e' = LitUnit ∧ ef = Some e);
+    last first.
+  - intros σ1 e2 σ2 ef Hstep%prim_ectx_step; last first.
+    { do 3 eexists. eapply ForkS. }
+    inversion_clear Hstep. done.
+  - intros ?. do 3 eexists. exists EmptyCtx. do 2 eexists.
+    split_ands; try (by rewrite fill_empty); [].
+    eapply ForkS.
+  - reflexivity.
+  - apply later_mono.
+    apply forall_intro=>e2. apply forall_intro=>ef.
+    apply impl_intro_l. apply const_elim_l. intros [-> ->].
+    (* FIXME RJ This is ridicolous. *)
+    transitivity (True ★ wp coPset_all e (λ _ : ival Σ, True))%I;
+      first by rewrite left_id.
+    apply sep_mono; last reflexivity.
+    rewrite -wp_value'; reflexivity.
 Qed.
